Remove depth from post-verifyrule definitions

theories/Checkloops.v
@@ -9,274 +9,140 @@ From Peg Require Import Verifyrule.
 (** CheckLoops predicate **)
 (** Check whether a pattern has potential infinite loops **)
 
-Inductive checkloops : grammar -> pat -> nat -> option bool -> Prop :=
+Inductive checkloops : grammar -> pat -> bool -> Prop :=
   | CLEmpty :
-      forall g d,
-      checkloops g PEmpty d (Some false)
+      forall g,
+      checkloops g PEmpty false
   | CLSet :
-      forall g f d,
-      checkloops g (PSet f) d (Some false)
-  | CLSequenceNone :
-      forall g p1 p2 d,
-      checkloops g p1 d None ->
-      checkloops g (PSequence p1 p2) d None
-  | CLSequenceSomeTrue :
-      forall g p1 p2 d,
-      checkloops g p1 d (Some true) ->
-      checkloops g (PSequence p1 p2) d (Some true)
-  | CLSequenceSomeFalse :
-      forall g p1 p2 res d,
-      checkloops g p1 d (Some false) ->
-      checkloops g p2 d res ->
-      checkloops g (PSequence p1 p2) d res
-  | CLChoiceNone :
-      forall g p1 p2 d,
-      checkloops g p1 d None ->
-      checkloops g (PChoice p1 p2) d None
-  | CLChoiceSomeTrue :
-      forall g p1 p2 d,
-      checkloops g p1 d (Some true) ->
-      checkloops g (PChoice p1 p2) d (Some true)
-  | CLChoiceSomeFalse :
-      forall g p1 p2 d res,
-      checkloops g p1 d (Some false) ->
-      checkloops g p2 d res ->
-      checkloops g (PChoice p1 p2) d res
-  | CLRepetitionLR :
-      forall g p d,
-      nullable g p d None ->
-      checkloops g (PRepetition p) d None
+      forall g f,
+      checkloops g (PSet f) false
+  | CLSequenceTrue :
+      forall g p1 p2,
+      checkloops g p1 true ->
+      checkloops g (PSequence p1 p2) true
+  | CLSequenceFalse :
+      forall g p1 p2 b,
+      checkloops g p1 false ->
+      checkloops g p2 b ->
+      checkloops g (PSequence p1 p2) b
+  | CLChoiceTrue :
+      forall g p1 p2,
+      checkloops g p1 true ->
+      checkloops g (PChoice p1 p2) true
+  | CLChoiceFalse :
+      forall g p1 p2 b,
+      checkloops g p1 false ->
+      checkloops g p2 b ->
+      checkloops g (PChoice p1 p2) b
   | CLRepetitionNullable :
-      forall g p d,
-      nullable g p d (Some true) ->
-      checkloops g (PRepetition p) d (Some true)
+      forall g p,
+      nullable g p true ->
+      checkloops g (PRepetition p) true
   | CLRepetitionNotNullable :
-      forall g p d res,
-      nullable g p d (Some false) ->
-      checkloops g p d res ->
-      checkloops g (PRepetition p) d res
+      forall g p b,
+      nullable g p false ->
+      checkloops g p b ->
+      checkloops g (PRepetition p) b
   | CLNot :
-      forall g p d res,
-      checkloops g p d res ->
-      checkloops g (PNot p) d res
+      forall g p b,
+      checkloops g p b ->
+      checkloops g (PNot p) b
   | CLNT :
-      forall g i d,
-      checkloops g (PNT i) d (Some false)
+      forall g i,
+      checkloops g (PNT i) false
   .
 
 Theorem checkloops_determinism :
-  forall g p d b1 b2,
-  checkloops g p d b1 ->
-  checkloops g p d b2 ->
+  forall g p b1 b2,
+  checkloops g p b1 ->
+  checkloops g p b2 ->
   b1 = b2.
 Proof.
   intros * H1 H2.
   generalize dependent b2.
   induction H1; intros;
   inversion H2; subst;
-  try assert (Some true = Some false) by auto;
-  try assert (Some false = Some true) by auto;
-  try assert (Some false = None) by auto;
-  try assert (None = Some false) by auto;
   try pose_nullable_determinism;
+  try assert (true = false) by auto;
+  try assert (false = true) by auto;
   try discriminate;
   auto.
 Qed.
 
 Ltac pose_checkloops_determinism :=
   match goal with
-    [ Hx1: checkloops ?g ?p ?d ?res1,
-      Hx2: checkloops ?g ?p ?d ?res2 |- _ ] =>
-          assert (res1 = res2)
+    [ Hx1: checkloops ?g ?p ?b1,
+      Hx2: checkloops ?g ?p ?b2 |- _ ] =>
+          assert (b1 = b2)
           by eauto using checkloops_determinism;
           clear Hx2
   end.
 
-Theorem checkloops_Some_S_depth :
-  forall g p d b,
-  checkloops g p d (Some b) ->
-  checkloops g p (S d) (Some b).
-Proof.
-  intros * H.
-  remember (Some b) as res.
-  generalize dependent b.
-  induction H;
-  intros;
-  try destruct1;
-  try discriminate;
-  eauto using checkloops, nullable_Some_S_depth.
-Qed.
-
-Theorem checkloops_Some_depth_le :
-  forall g p d d' b,
-  checkloops g p d (Some b) ->
-  d <= d' ->
-  checkloops g p d' (Some b).
-Proof.
-  intros * H Hle.
-  induction Hle;
-  eauto using checkloops_Some_S_depth.
-Qed.
-
-Lemma checkloops_Some_determinism :
-  forall g p d1 d2 b1 b2,
-  checkloops g p d1 (Some b1) ->
-  checkloops g p d2 (Some b2) ->
-  b1 = b2.
-Proof.
-  intros * H1 H2.
-  destruct (Compare_dec.le_ge_dec d1 d2);
-  try match goal with
-    [ Hge: ?x >= ?y |- _ ] =>
-        assert (y <= x) by lia
-  end;
-  match goal with
-    [ Hx: checkloops ?g ?p ?dx (Some ?bx),
-      Hle: ?dx <= ?dy |- _ ] =>
-          assert (checkloops g p dy (Some bx))
-          by eauto using checkloops_Some_depth_le
-  end;
-  match goal with
-    [ Hx1: checkloops ?g ?p ?d (Some ?b1),
-      Hx2: checkloops ?g ?p ?d (Some ?b2) |- _ ] =>
-          assert (Some b1 = Some b2)
-          by eauto using checkloops_determinism
-  end;
-  destruct1;
-  auto.
-Qed.
-
 Lemma checkloops_safe_grammar :
   forall g p,
-  (forall r, In r g -> coherent g r true) ->
-  (forall r nb, In r g -> exists d b k, verifyrule g r d nb (Some b) k) ->
+  lcoherent g g true ->
+  lverifyrule g g true ->
   coherent g p true ->
-  exists d b, checkloops g p d (Some b).
+  exists b, checkloops g p b.
 Proof.
   intros * Hgc Hgv Hpc.
   induction p;
   inversion Hpc; subst;
-  repeat specialize_coherent;
-  repeat destruct_exists_hyp;
   try match goal with
-    [ Hx1: checkloops ?g ?p1 ?d1 (Some ?b1),
-      Hx2: checkloops ?g ?p2 ?d2 (Some ?b2)
-      |- exists _ _, checkloops ?g (_ ?p1 ?p2) _ _ ] =>
-          assert (d1 <= d1 + d2) by lia;
-          assert (d2 <= d1 + d2) by lia;
-          assert (checkloops g p1 (d1 + d2) (Some b1))
-          by eauto using checkloops_Some_depth_le;
-          assert (checkloops g p2 (d1 + d2) (Some b2))
-          by eauto using checkloops_Some_depth_le;
-          destruct b1;
-          eauto using checkloops;
-          fail
+    [ |- exists b, checkloops ?g (_ ?p1 ?p2) b ] =>
+        assert (exists b, checkloops g p1 b) as [[|] ?] by eauto;
+        assert (exists b, checkloops g p2 b) as [? ?] by eauto
   end;
   try match goal with
-    [ Hx: coherent ?g ?p true,
-      Hy: checkloops ?g ?p ?d' (Some ?b')
-      |- exists _ _, checkloops ?g (PRepetition ?p) _ _ ] =>
-          assert (exists d b k, verifyrule g p d false (Some b) k)
-          as [d [b [k ?]]] by eauto using verifyrule_safe_grammar_yields_safe_pattern;
-          assert (nullable g p d (Some b))
-          by eauto using verifyrule_similar_to_nullable;
-          assert (d <= d + d') by lia;
-          assert (d' <= d + d') by lia;
-          assert (nullable g p (d + d') (Some b))
-          by eauto using nullable_Some_depth_le;
-          assert (checkloops g p (d + d') (Some b'))
-          by eauto using checkloops_Some_depth_le;
-          destruct b;
-          eauto using checkloops;
-          fail
+    [ |- exists b, checkloops ?g (_ ?p) b ] =>
+        assert (exists b, checkloops g p b) as [? ?] by eauto
   end;
   try match goal with
-    [ Hx: checkloops ?g ?p ?d (Some _)
-      |- exists _ _, checkloops ?g (_ ?p) _ _ ] =>
-          exists d;
-          eauto using checkloops;
-          fail
+    [ |- exists bx, checkloops ?g (PRepetition ?p) bx ] =>
+        assert (exists d b k, verifyrule g p d false (Some b) k)
+        as [d [b [k ?]]] by eauto using
+        verifyrule_safe_grammar_yields_safe_pattern,
+        lcoherent_true_In,
+        lverifyrule_true_In;
+        assert (nullable g p b)
+        by eauto using verifyrule_similar_to_nullable;
+        destruct b
   end;
-  try (exists 1; eauto using checkloops; fail).
-Qed.
-
-Lemma checkloops_convergence :
-  forall g p d d' res,
-  (forall r, In r g -> coherent g r true) ->
-  (forall r nb, In r g -> exists d b k, verifyrule g r d nb (Some b) k) ->
-  coherent g p true ->
-  length g < d ->
-  checkloops g p d res ->
-  d <= d' ->
-  checkloops g p d' res.
-Proof.
-  intros * Hgc Hgv Hpc Hlt Hcl Hle.
-  generalize dependent d'.
-  induction Hcl;
-  intros;
-  inversion Hpc; subst;
-  eauto using checkloops, nullable_convergence.
-Qed.
-
-Lemma checkloops_Some_convergence :
-  forall g p d d' b res,
-  (forall r, In r g -> coherent g r true) ->
-  (forall r nb, In r g -> exists d b k, verifyrule g r d nb (Some b) k) ->
-  coherent g p true ->
-  checkloops g p d (Some b) ->
-  length g < d' ->
-  checkloops g p d' res ->
-  res = Some b.
-Proof.
-  intros * Hgc Hgv Hpc Hc Hlt Hc'.
-  destruct (Compare_dec.le_ge_dec d d');
-  match goal with
-  | [ _: ?d <= ?d' |- _ ] =>
-      assert (checkloops g p d' (Some b))
-      by eauto using checkloops_Some_depth_le
-  | [ _: ?d >= ?d' |- _ ] =>
-      assert (d' <= d) by lia;
-      assert (checkloops g p d res)
-      by eauto using checkloops_convergence
-  end;
-  pose_checkloops_determinism;
-  subst;
-  eauto.
+  eauto using checkloops.
 Qed.
 
 (** CheckLoops function **)
 
-Fixpoint checkloops_comp g p d gas {struct gas} :=
+Fixpoint checkloops_comp g p gas {struct gas} :=
   match gas with
   | O => None
   | S gas' => match p with
-              | PEmpty => Some (Some false)
-              | PSet _ => Some (Some false)
-              | PSequence p1 p2 => match checkloops_comp g p1 d gas' with
-                                   | Some (Some false) => checkloops_comp g p2 d gas'
-                                   | res => res
+              | PEmpty => Some false
+              | PSet _ => Some false
+              | PSequence p1 p2 => match checkloops_comp g p1 gas' with
+                                   | Some false => checkloops_comp g p2 gas'
+                                   | ob => ob
                                    end
-              | PChoice p1 p2 => match checkloops_comp g p1 d gas' with
-                                 | Some (Some false) => checkloops_comp g p2 d gas'
-                                 | res => res
+              | PChoice p1 p2 => match checkloops_comp g p1 gas' with
+                                 | Some false => checkloops_comp g p2 gas'
+                                 | ob => ob
                                  end
-              | PRepetition p' => match nullable_comp g p' d gas' with
-                                  | Some (Some false) => checkloops_comp g p' d gas'
-                                  | res => res
+              | PRepetition p' => match nullable_comp g p' gas' with
+                                  | Some false => checkloops_comp g p' gas'
+                                  | ob => ob
                                   end
-              | PNot p' => checkloops_comp g p' d gas'
-              | PNT _ => Some (Some false)
+              | PNot p' => checkloops_comp g p' gas'
+              | PNT _ => Some false
               end
   end.
 
 Lemma checkloops_comp_soundness :
-  forall g p d gas res,
-  checkloops_comp g p d gas = Some res ->
-  checkloops g p d res.
+  forall g p gas b,
+  checkloops_comp g p gas = Some b ->
+  checkloops g p b.
 Proof.
   intros * H.
-  generalize dependent res.
-  generalize dependent d.
+  generalize dependent b.
   generalize dependent p.
   generalize dependent g.
   induction gas; try discriminate; intros.
@@ -289,13 +155,12 @@ Proof.
 Qed.
 
 Lemma checkloops_comp_S_gas :
-  forall g p d gas res,
-  checkloops_comp g p d gas = Some res ->
-  checkloops_comp g p d (S gas) = Some res.
+  forall g p gas b,
+  checkloops_comp g p gas = Some b ->
+  checkloops_comp g p (S gas) = Some b.
 Proof.
   intros * H.
-  generalize dependent res.
-  generalize dependent d.
+  generalize dependent b.
   generalize dependent p.
   generalize dependent g.
   induction gas; try discriminate; intros.
@@ -306,11 +171,11 @@ Proof.
   try discriminate;
   remember (S gas) as gas';
   repeat match goal with
-    [ Hx: checkloops_comp _ _ _ gas = Some _ |- _ ] =>
+    [ Hx: checkloops_comp _ _ gas = Some _ |- _ ] =>
         apply IHgas in Hx
   end;
   try match goal with
-    [ Hx: nullable_comp _ _ _ gas = Some _ |- _ ] =>
+    [ Hx: nullable_comp _ _ gas = Some _ |- _ ] =>
         apply nullable_comp_S_gas in Hx
   end;
   simpl;
@@ -320,40 +185,42 @@ Proof.
 Qed.
 
 Lemma checkloops_comp_le_gas :
-  forall g p d gas gas' res,
-  checkloops_comp g p d gas = Some res ->
+  forall g p gas gas' b,
+  checkloops_comp g p gas = Some b ->
   gas <= gas' ->
-  checkloops_comp g p d gas' = Some res.
+  checkloops_comp g p gas' = Some b.
 Proof.
   intros * H Hle.
   induction Hle;
   eauto using checkloops_comp_S_gas.
 Qed.
 
-Lemma checkloops_comp_termination :
-  forall g p d,
-  (forall r, In r g -> coherent g r true) ->
+Lemma checkloops_comp_gas_exists :
+  forall g p,
+  lcoherent g g true ->
+  lverifyrule g g true ->
   coherent g p true ->
-  exists gas res,
-  checkloops_comp g p d gas = Some res.
+  exists gas b,
+  checkloops_comp g p gas = Some b.
 Proof.
-  intros * Hgc Hpc.
+  intros * Hgc Hgv Hpc.
   induction p; intros;
   inversion Hpc; subst;
   repeat specialize_coherent;
   repeat destruct_exists_hyp;
   (* 2 recursive calls *)
   try match goal with
-    [ Hx1: checkloops_comp ?g ?p1 ?d ?gas1 = Some ?res1,
-      Hx2: checkloops_comp ?g ?p2 ?d ?gas2 = Some ?res2 |- _ ] =>
-          assert (gas1 <= gas1 + gas2) by lia;
-          assert (gas2 <= gas1 + gas2) by lia;
-          assert (checkloops_comp g p1 d (gas1 + gas2) = Some res1)
+    [ Hx1: checkloops_comp ?g ?p1 ?gas1 = Some ?b1,
+      Hx2: checkloops_comp ?g ?p2 ?gas2 = Some ?b2 |- _ ] =>
+          pose (gas1 + gas2) as gas;
+          assert (gas1 <= gas) by lia;
+          assert (gas2 <= gas) by lia;
+          assert (checkloops_comp g p1 gas = Some b1)
           as Hx1' by eauto using checkloops_comp_le_gas;
-          assert (checkloops_comp g p2 d (gas1 + gas2) = Some res2)
+          assert (checkloops_comp g p2 gas = Some b2)
           by eauto using checkloops_comp_le_gas;
-          exists (1 + gas1 + gas2);
-          destruct res1 as [[|]|];
+          exists (S gas);
+          destruct b1;
           simpl;
           rewrite Hx1';
           eauto;
@@ -361,26 +228,32 @@ Proof.
   end;
   (* 1 recursive call + nullable_comp *)
   try match goal with
-    [ Hx1: checkloops_comp ?g ?p1 ?d ?gas1 = Some ?res1 |- _ ] =>
-        assert (exists gas res, nullable_comp g p1 d gas = Some res)
-        as [gas2 [res2 ?]] by eauto using nullable_comp_termination;
-        assert (gas1 <= gas1 + gas2) by lia;
-        assert (gas2 <= gas1 + gas2) by lia;
-        assert (checkloops_comp g p1 d (gas1 + gas2) = Some res1)
+    [ Hx1: checkloops_comp ?g ?p1 ?gas1 = Some ?b1 |- _ ] =>
+        assert (exists d b k, verifyrule g p1 d false (Some b) k)
+        as [d [b [k ?]]] by eauto using
+        verifyrule_safe_grammar_yields_safe_pattern,
+        lcoherent_true_In,
+        lverifyrule_true_In;
+        assert (exists gas, nullable_comp g p1 gas = Some b)
+        as [gas2 ?] by eauto using nullable_comp_gas_bounded;
+        pose (gas1 + gas2) as gas;
+        assert (gas1 <= gas) by lia;
+        assert (gas2 <= gas) by lia;
+        assert (checkloops_comp g p1 gas = Some b1)
         as Hx1' by eauto using checkloops_comp_le_gas;
-        assert (nullable_comp g p1 d (gas1 + gas2) = Some res2)
+        assert (nullable_comp g p1 gas = Some b)
         as Hx2' by eauto using nullable_comp_le_gas;
-        exists (1 + gas1 + gas2);
+        exists (S gas);
         simpl;
         rewrite Hx2';
-        destruct res2 as [[|]|];
+        destruct b;
         eauto;
         fail
   end;
   (* 1 recursive call *)
   try match goal with
-    [ Hx1: checkloops_comp ?g ?p1 ?d ?gas1 = Some ?res1 |- _ ] =>
-        exists (1 + gas1);
+    [ Hx1: checkloops_comp ?g ?p1 ?gas1 = Some ?b1 |- _ ] =>
+        exists (S gas1);
         simpl;
         eauto;
         fail
@@ -389,59 +262,63 @@ Proof.
   try (exists 1; simpl; eauto; fail).
 Qed.
 
-Ltac specialize_checkloops :=
-  match goal with
-    [ Hx: checkloops ?g ?p _ ?b, IHx: forall d, checkloops ?g ?p d ?b -> _ |- _ ] =>
-        specialize (IHx _ Hx)
-  end.
-
 Lemma checkloops_comp_gas_bounded :
-  forall g p gas d,
-  (forall r, In r g -> coherent g r true) ->
+  forall g p gas,
+  lcoherent g g true ->
   coherent g p true ->
-  gas >= pat_size p + d * (grammar_size g) ->
-  exists res,
-  checkloops_comp g p d gas = Some res.
+  lverifyrule g g true ->
+  gas >= pat_size p + S (Datatypes.length g) * (grammar_size g) ->
+  exists b, checkloops_comp g p gas = Some b.
 Proof.
-  intros * Hgc Hpc Hge.
+  intros * Hlc Hc Hlv Hge.
   generalize dependent gas.
   induction p; intros;
-  inversion Hpc; subst;
+  inversion Hc; subst;
   simpl in Hge;
   destruct gas;
   try match goal with
     [ Hx: 0 >= S _ |- _ ] =>
         inversion Hx
   end;
-  try match goal with
-    [ |- exists _, _ ?g (_ ?p) ?d (S ?gas) = _ ] =>
-        assert (gas >= pat_size p + d * grammar_size g) by lia
-  end;
-  try match goal with
-    [ |- exists _, _ ?g (_ ?p _) ?d (S ?gas) = _ ] =>
-        assert (gas >= pat_size p + d * grammar_size g) by lia
-  end;
-  simpl;
-  eauto.
-  - (* PSequence p1 p2 *)
-    assert (exists res, checkloops_comp g p1 d gas = Some res)
-    as [res1 Hclp1] by eauto.
-    assert (exists res, checkloops_comp g p2 d gas = Some res)
-    as [? ?] by eauto.
-    rewrite Hclp1.
-    destruct res1 as [[|]|]; eauto.
-  - (* PChoice p1 p2 *)
-    assert (exists res, checkloops_comp g p1 d gas = Some res)
-    as [res1 Hclp1] by eauto.
-    assert (exists res, checkloops_comp g p2 d gas = Some res)
-    as [? ?] by eauto.
-    rewrite Hclp1.
-    destruct res1 as [[|]|]; eauto.
-  - (* PRepetition p *)
-    assert (exists res, nullable_comp g p d gas = Some res)
-    as [res Hnp] by eauto using nullable_comp_gas_bounded.
-    rewrite Hnp.
-    destruct res as [[|]|]; eauto.
+  (* PEmpty, PSet f, PNT i *)
+  try (simpl; eauto; fail);
+  (* PNot p *)
+  try (
+    assert (gas >= pat_size p + S (length g) * grammar_size g) by lia;
+    eauto;
+    fail
+  );
+  (* PSequence p1 p2, PChoice p1 p2 *)
+  try (
+    assert (gas >= pat_size p1 + S (length g) * grammar_size g) by lia;
+    assert (gas >= pat_size p2 + S (length g) * grammar_size g) by lia;
+    assert (exists b, checkloops_comp g p1 gas = Some b)
+    as [bc1 Hc1] by eauto;
+    simpl;
+    rewrite Hc1;
+    destruct bc1;
+    eauto;
+    fail
+  );
+  (* PRepetition p *)
+  try (
+    assert (exists d b k, verifyrule g p d false (Some b) k)
+    as [? [bv [? ?]]] by eauto using
+    verifyrule_safe_grammar_yields_safe_pattern,
+    lcoherent_true_In,
+    lverifyrule_true_In;
+    assert (gas >= pat_size p + S (Datatypes.length g) * grammar_size g) by lia;
+    assert (nullable_comp g p gas = Some bv)
+    as Hn by eauto using nullable_comp_gas_bounded;
+    assert (gas >= pat_size p + S (length g) * grammar_size g) by lia;
+    assert (exists b, checkloops_comp g p gas = Some b)
+    as [bc' Hc'] by eauto;
+    simpl;
+    rewrite Hn;
+    destruct bv;
+    eauto;
+    fail
+  ).
 Qed.
 
 (** CheckLoops for lists of patterns
@@ -458,12 +335,12 @@ Inductive lcheckloops : grammar -> list pat -> bool -> Prop :=
       forall g,
       lcheckloops g nil false
   | LCLConsSomeTrue :
-      forall g r d rs,
-      checkloops g r d (Some true) ->
+      forall g r rs,
+      checkloops g r true ->
       lcheckloops g (cons r rs) true
   | LCLConsSomeFalse :
-      forall g r d rs b,
-      checkloops g r d (Some false) ->
+      forall g r rs b,
+      checkloops g r false ->
       lcheckloops g rs b ->
       lcheckloops g (cons r rs) b
   .
@@ -479,10 +356,10 @@ Proof.
   induction H1; intros;
   inversion H2; subst;
   try match goal with
-    [ Hx1: checkloops ?g ?r ?d1 (Some ?b1),
-      Hx2: checkloops ?g ?r ?d2 (Some ?b2) |- _ ] =>
+    [ Hx1: checkloops ?g ?r ?b1,
+      Hx2: checkloops ?g ?r ?b2 |- _ ] =>
           assert (b1 = b2)
-          by eauto using checkloops_Some_determinism
+          by eauto using checkloops_determinism
   end;
   try discriminate;
   auto.
@@ -492,8 +369,7 @@ Lemma lcheckloops_false_In :
   forall g rs r,
   lcheckloops g rs false ->
   In r rs ->
-  exists d,
-  checkloops g r d (Some false).
+  checkloops g r false.
 Proof.
   intros * Hcl HIn.
   generalize dependent r.
@@ -514,10 +390,10 @@ Qed.
 Fixpoint lcheckloops_comp g rs gas :=
   match rs with
   | nil => Some false
-  | cons r rs' => match checkloops_comp g r (S (length g)) gas with
-                  | Some (Some false) => lcheckloops_comp g rs' gas
-                  | Some (Some true) => Some true
-                  | _ => None
+  | cons r rs' => match checkloops_comp g r gas with
+                  | Some false => lcheckloops_comp g rs' gas
+                  | Some true => Some true
+                  | None => None
                   end
   end.
 
@@ -539,12 +415,12 @@ Proof.
   - (* cons r rs *)
     match goal with
       [ Hx: match ?x with | _ => _ end = _ |- _ ] =>
-          destruct x as [[[|]|]|] eqn:?;
+          destruct x as [[|]|] eqn:?;
           try destruct1;
           try discriminate;
           try match goal with
-            [ Hx: checkloops_comp ?g ?r ?d ?gas = Some ?res |- _ ] =>
-                assert (checkloops g r d res)
+            [ Hx: checkloops_comp ?g ?r ?gas = Some ?b |- _ ] =>
+                assert (checkloops g r b)
                 by eauto using checkloops_comp_soundness
           end;
           eauto using lcheckloops
@@ -569,12 +445,12 @@ Proof.
   - (* cons r rs *)
     match goal with
       [ Hx: match ?x with | _ => _ end = _ |- _ ] =>
-          destruct x as [[[|]|]|] eqn:?;
+          destruct x as [[|]|] eqn:?;
           try discriminate;
           try destruct1;
           try match goal with
-            [ Hx: checkloops_comp ?g ?r ?d ?gas = Some ?res |- _ ] =>
-                assert (checkloops_comp g r d (S gas) = Some res)
+            [ Hx: checkloops_comp ?g ?r ?gas = Some ?b |- _ ] =>
+                assert (checkloops_comp g r (S gas) = Some b)
                 as ? by eauto using checkloops_comp_S_gas;
                 unfold lcheckloops_comp;
                 rewrite_match_subject_in_goal;
@@ -595,7 +471,7 @@ Proof.
   eauto using lcheckloops_comp_S_gas.
 Qed.
 
-Lemma lcheckloops_comp_termination :
+Lemma lcheckloops_comp_gas_exists :
   forall g rs,
   lcoherent g g true ->
   lcoherent g rs true ->
@@ -612,31 +488,24 @@ Proof.
     eauto.
   - (* cons r rs *)
     inversion Hrsc; subst.
-    match goal with
-      [ Hx: lcoherent ?g ?rs true -> _, Hy: lcoherent ?g ?rs true |- _ ] =>
-          specialize (Hx Hy) as [gas1 [resrs ?]]
-    end.
-    assert (exists d b, checkloops g r d (Some b))
-    as [d [b ?]]
-    by eauto using checkloops_safe_grammar, lcoherent_true_In, lverifyrule_true_In.
-    assert (exists gas res, checkloops_comp g r (S (length g)) gas = Some res)
-    as [gas2 [res Hcl]]
-    by eauto using checkloops_comp_termination, lcoherent_true_In.
-    assert (checkloops g r (S (length g)) res)
+    assert (exists gas b, lcheckloops_comp g rs gas = Some b)
+    as [gaslcl [blcl ?]] by eauto.
+    assert (exists gas b, checkloops_comp g r gas = Some b)
+    as [gascl [bcl ?]]
+    by eauto using checkloops_comp_gas_exists, lcoherent_true_In.
+    assert (checkloops g r bcl)
     by eauto using checkloops_comp_soundness.
-    assert (res = Some b)
-    by eauto using checkloops_Some_convergence, lcoherent_true_In, lverifyrule_true_In.
-    subst res.
     simpl.
-    assert (gas1 <= gas1 + gas2) by lia.
-    assert (gas2 <= gas1 + gas2) by lia.
-    assert (lcheckloops_comp g rs (gas1 + gas2) = Some resrs)
+    pose (gaslcl + gascl) as gas.
+    assert (gaslcl <= gas) by lia.
+    assert (gascl <= gas) by lia.
+    assert (lcheckloops_comp g rs gas = Some blcl)
     as Hlcl' by eauto using lcheckloops_comp_le_gas.
-    assert (checkloops_comp g r (S (length g)) (gas1 + gas2) = Some (Some b))
+    assert (checkloops_comp g r gas = Some bcl)
     as Hcl' by eauto using checkloops_comp_le_gas.
-    exists (gas1 + gas2).
+    exists gas.
     rewrite Hcl'.
-    destruct b;
+    destruct bcl;
     eauto.
 Qed.
 
@@ -659,16 +528,10 @@ Proof.
   assert (gas >= grammar_size rs + S (length g) * grammar_size g) by lia.
   assert (exists b, lcheckloops_comp g rs gas = Some b) as [? ?] by eauto.
   assert (gas >= pat_size r + S (length g) * grammar_size g) by lia.
-  assert (exists b, checkloops_comp g r (S (length g)) gas = Some b)
-  as [clres Hcl] by eauto using checkloops_comp_gas_bounded, lcoherent_true_In.
+  assert (exists b, checkloops_comp g r gas = Some b)
+  as [clres Hcl]
+  by eauto using checkloops_comp_gas_bounded, lcoherent_true_In.
   rewrite Hcl.
-  assert (exists d b, checkloops g r d (Some b))
-  as [d [b ?]]
-  by eauto using checkloops_safe_grammar, lcoherent_true_In, lverifyrule_true_In.
-  assert (checkloops g r (S (length g)) clres)
-  by eauto using checkloops_comp_soundness.
-  assert (clres = Some b)
-  by eauto using checkloops_Some_convergence, lcoherent_true_In, lverifyrule_true_In.
-  subst clres.
-  destruct b; eauto.
+  destruct clres;
+  eauto.
 Qed.
