theories/Nullable.v
@@ -1,82 +1,70 @@
-From Coq Require Import Strings.String.
-From Coq Require Import Strings.Ascii.
-From Coq Require Import Lists.List.
+From Coq Require Import Bool.
 From Coq Require Import Lia.
+From Coq Require Import Lists.List.
+From Coq Require Import Strings.Ascii.
+From Coq Require Import Strings.String.
+From Peg Require Import Coherent.
+From Peg Require Import Match.
+From Peg Require Import Suffix.
 From Peg Require Import Syntax.
 From Peg Require Import Tactics.
-From Peg Require Import Match.
-From Peg Require Import Coherent.
 From Peg Require Import Verifyrule.
-From Peg Require Import Suffix.
 
 Import ListNotations.
+
 
 (** Nullable predicate **)
 (** A "nullable" pattern may match successfully without consuming any characters **)
 
-Inductive nullable : grammar -> pat -> nat -> option bool -> Prop :=
+Inductive nullable : grammar -> pat -> bool -> Prop :=
   | NEmpty :
-      forall g d,
-      nullable g PEmpty d (Some true)
+      forall g,
+      nullable g PEmpty true
   | NSet :
-      forall g f d,
-      nullable g (PSet f) d (Some false)
-  | NSequenceNone :
-      forall g p1 p2 d,
-      nullable g p1 d None ->
-      nullable g (PSequence p1 p2) d None
-  | NSequenceSomeFalse :
-      forall g p1 p2 d,
-      nullable g p1 d (Some false) ->
-      nullable g (PSequence p1 p2) d (Some false)
-  | NSequenceSomeTrue :
-      forall g p1 p2 d res,
-      nullable g p1 d (Some true) ->
-      nullable g p2 d res ->
-      nullable g (PSequence p1 p2) d res
-  | NChoiceNone :
-      forall g p1 p2 d,
-      nullable g p1 d None ->
-      nullable g (PChoice p1 p2) d None
-  | NChoiceSomeFalse :
-      forall g p1 p2 d res,
-      nullable g p1 d (Some false) ->
-      nullable g p2 d res ->
-      nullable g (PChoice p1 p2) d res
-  | NChoiceSomeTrue :
-      forall g p1 p2 d,
-      nullable g p1 d (Some true) ->
-      nullable g (PChoice p1 p2) d (Some true)
+      forall g f,
+      nullable g (PSet f) false
+  | NSequence1 :
+      forall g p1 p2,
+      nullable g p1 false ->
+      nullable g (PSequence p1 p2) false
+  | NSequence2 :
+      forall g p1 p2 b,
+      nullable g p1 true ->
+      nullable g p2 b ->
+      nullable g (PSequence p1 p2) b
+  | NChoice1 :
+      forall g p1 p2,
+      nullable g p1 true ->
+      nullable g (PChoice p1 p2) true
+  | NChoice :
+      forall g p1 p2 b,
+      nullable g p1 false ->
+      nullable g p2 b ->
+      nullable g (PChoice p1 p2) b
   | NRepetition :
-      forall g p d,
-      nullable g (PRepetition p) d (Some true)
+      forall g p,
+      nullable g (PRepetition p) true
   | NNot :
-      forall g p d,
-      nullable g (PNot p) d (Some true)
-  | NNTZero :
-      forall g i p,
+      forall g p,
+      nullable g (PNot p) true
+  | NNT :
+      forall g i p b,
       nth_error g i = Some p ->
-      nullable g (PNT i) O None
-  | NNTSucc :
-      forall g i p res d,
-      nth_error g i = Some p ->
-      nullable g p d res ->
-      nullable g (PNT i) (S d) res
+      nullable g p b ->
+      nullable g (PNT i) b
   .
 
 (* ! {A <- A} |= A *)
 Example nullable_ex1 :
-  forall d b,
+  forall b,
     ~ nullable
     [PNT 0]
     (PNT 0)
-    d
-    (Some b).
+    b.
 Proof.
   intros * H.
   remember (PNT 0) as p.
   remember [p] as g.
-  remember (Some b) as res.
   induction H;
   try discriminate;
   try destruct1;
@@ -87,20 +75,19 @@ Qed.
 
 (* G |= ε *)
 Example nullable_ex2 :
-  forall g d,
-  nullable g PEmpty d (Some true).
+  forall g,
+  nullable g PEmpty true.
 Proof.
   intros.
   eauto using nullable.
 Qed.
 
-Example dot_charset : (ascii -> bool) :=
-  (fun _ => true).
+Example PDot : pat := PSet (fun _ => true).
 
 (* ! G |= . *)
 Example nullable_ex3 :
-  forall g d,
-  nullable g (PSet dot_charset) d (Some false).
+  forall g,
+  nullable g PDot false.
 Proof.
   intros.
   eauto using nullable.
@@ -108,8 +95,8 @@ Qed.
 
 (* G |= ε ε *)
 Example nullable_ex5 :
-  forall g d,
-  nullable g (PSequence PEmpty PEmpty) d (Some true).
+  forall g,
+  nullable g (PSequence PEmpty PEmpty) true.
 Proof.
   intros.
   eauto using nullable.
@@ -117,8 +104,8 @@ Qed.
 
 (* ! G |= . ε *)
 Example nullable_ex6 :
-  forall g d,
-  nullable g (PSequence (PSet dot_charset) PEmpty) d (Some false).
+  forall g,
+  nullable g (PSequence PDot PEmpty) false.
 Proof.
   intros.
   eauto using nullable.
@@ -126,8 +113,8 @@ Qed.
 
 (* ! G |= ε . *)
 Example nullable_ex7 :
-  forall g d,
-  nullable g (PSequence PEmpty (PSet dot_charset)) d (Some false).
+  forall g,
+  nullable g (PSequence PEmpty PDot) false.
 Proof.
   intros.
   eauto using nullable.
@@ -135,8 +122,8 @@ Qed.
 
 (* ! G |= . . *)
 Example nullable_ex8 :
-  forall g d,
-  nullable g (PSequence (PSet dot_charset) (PSet dot_charset)) d (Some false).
+  forall g,
+  nullable g (PSequence PDot PDot) false.
 Proof.
   intros.
   eauto using nullable.
@@ -144,8 +131,8 @@ Qed.
 
 (* G |= ε / ε *)
 Example nullable_ex9 :
-  forall g d,
-  nullable g (PChoice PEmpty PEmpty) d (Some true).
+  forall g,
+  nullable g (PChoice PEmpty PEmpty) true.
 Proof.
   intros.
   eauto using nullable.
@@ -153,8 +140,8 @@ Qed.
 
 (* G |= . / ε *)
 Example nullable_ex10 :
-  forall g d,
-  nullable g (PChoice (PSet dot_charset) PEmpty) d (Some true).
+  forall g,
+  nullable g (PChoice PDot PEmpty) true.
 Proof.
   intros.
   eauto using nullable.
@@ -162,8 +149,8 @@ Qed.
 
 (* G |= ε / . *)
 Example nullable_ex11 :
-  forall g d,
-  nullable g (PChoice PEmpty (PSet dot_charset)) d (Some true).
+  forall g,
+  nullable g (PChoice PEmpty PDot) true.
 Proof.
   intros.
   eauto using nullable.
@@ -171,8 +158,8 @@ Qed.
 
 (* ! G |= . / . *)
 Example nullable_ex12 :
-  forall g d,
-  nullable g (PChoice (PSet dot_charset) (PSet dot_charset)) d (Some false).
+  forall g,
+  nullable g (PChoice PDot PDot) false.
 Proof.
   intros.
   eauto using nullable.
@@ -180,8 +167,8 @@ Qed.
 
 (* G |= p* *)
 Example nullable_ex13 :
-  forall g p d,
-  nullable g (PRepetition p) d (Some true).
+  forall g p,
+  nullable g (PRepetition p) true.
 Proof.
   intros.
   eauto using nullable.
@@ -189,8 +176,8 @@ Qed.
 
 (* G |= !p *)
 Example nullable_ex14 :
-  forall g p d,
-  nullable g (PNot p) d (Some true).
+  forall g p,
+  nullable g (PNot p) true.
 Proof.
   intros.
   eauto using nullable.
@@ -198,12 +185,10 @@ Qed.
 
 (* ! { P <- . P } |= P *)
 Example nullable_ex15 :
-  forall d,
   nullable
-    [PSequence (PSet dot_charset) (PNT 0)]
+    [PSequence PDot (PNT 0)]
     (PNT 0)
-    (S d)
-    (Some false).
+    false.
 Proof.
   intros.
   econstructor; simpl; eauto.
@@ -212,12 +197,10 @@ Qed.
 
 (* { P <- . P / ε } |= P *)
 Example nullable_ex16 :
-  forall d,
   nullable
-    [PChoice (PSequence (PSet dot_charset) (PNT 0)) PEmpty]
+    [PChoice (PSequence PDot (PNT 0)) PEmpty]
     (PNT 0)
-    (S d)
-    (Some true).
+    true.
 Proof.
   intros.
   econstructor; simpl; eauto.
@@ -226,8 +209,8 @@ Qed.
 
 (* ! {} |= A *)
 Example nullable_ex17 :
-  forall d res,
-  ~ nullable [] (PNT 0) d res.
+  forall b,
+  ~ nullable [] (PNT 0) b.
 Proof.
   intros * H.
   inversion H;
@@ -237,37 +220,35 @@ Qed.
 
 (* { A <- . A | ε ; B <- A A } |= A B *)
 Example nullable_ex18 :
-  forall d,
   nullable
-  [PChoice (PSequence (PSet dot_charset) (PNT 0)) PEmpty; PSequence (PNT 0) (PNT 0)]
+  [PChoice (PSequence PDot (PNT 0)) PEmpty; PSequence (PNT 0) (PNT 0)]
   (PSequence (PNT 0) (PNT 1))
-  (S (S d))
-  (Some true).
+  true.
 Proof.
   intros.
   repeat match goal with
-         | [ |- nullable _ (PSequence _ _) _ _ ] => econstructor
-         | [ |- nullable _ (PNT _) _ _ ] => econstructor; simpl; eauto
-         | [ |- nullable _ (PChoice _ _) _ _ ] => eauto using nullable
+         | [ |- nullable _ (PSequence _ _) _ ] => econstructor
+         | [ |- nullable _ (PNT _) _ ] => econstructor; simpl; eauto
+         | [ |- nullable _ (PChoice _ _) _ ] => eauto using nullable
          | _ => fail
          end.
 Qed.
 
 Lemma nullable_determinism :
-  forall g p d res1 res2,
-  nullable g p d res1 ->
-  nullable g p d res2 ->
-  res1 = res2.
+  forall g p b1 b2,
+  nullable g p b1 ->
+  nullable g p b2 ->
+  b1 = b2.
 Proof.
   intros * H1 H2.
-  generalize dependent res2.
+  generalize dependent b2.
   induction H1;
   intros;
   inversion H2; subst;
   try destruct2sep;
   try match goal with
-  [ IHx: forall resx, nullable ?g ?p ?d resx -> ?res1 = resx,
-    Hx: nullable ?g ?p ?d ?res2 |- _ ] =>
+  [ IHx: forall bx, nullable ?g ?p bx -> ?b1 = bx,
+    Hx: nullable ?g ?p ?b2 |- _ ] =>
         apply IHx in Hx;
         discriminate
   end;
@@ -276,69 +257,17 @@ Qed.
 
 Ltac pose_nullable_determinism :=
   match goal with
-    [ Hx1: nullable ?g ?p ?d ?res1,
-      Hx2: nullable ?g ?p ?d ?res2 |- _ ] =>
-          assert (res1 = res2)
-          by eauto using nullable_determinism;
-          clear Hx2
-  end.
-
-Lemma nullable_Some_S_depth :
-  forall g p d b,
-  nullable g p d (Some b) ->
-  nullable g p (S d) (Some b).
-Proof.
-  intros * H.
-  remember (Some b) as res.
-  generalize dependent b.
-  induction H; intros;
-  try discriminate;
-  eauto using nullable.
-Qed.
-
-Lemma nullable_Some_depth_le :
-  forall g p d d' b,
-  nullable g p d (Some b) ->
-  d <= d' ->
-  nullable g p d' (Some b).
-Proof.
-  intros * H Hle.
-  induction Hle;
-  eauto using nullable_Some_S_depth.
-Qed.
-
-Lemma nullable_Some_determinism :
-  forall g p d1 d2 b1 b2,
-  nullable g p d1 (Some b1) ->
-  nullable g p d2 (Some b2) ->
-  b1 = b2.
-Proof.
-  intros.
-  pose (d1 + d2) as dsum.
-  assert (d1 <= dsum) by lia.
-  assert (d2 <= dsum) by lia.
-  assert (nullable g p dsum (Some b1))
-  by eauto using nullable_Some_depth_le.
-  assert (nullable g p dsum (Some b2))
-  by eauto using nullable_Some_depth_le.
-  pose_nullable_determinism.
-  destruct1.
-  eauto.
-Qed.
-
-Ltac pose_nullable_Some_determinism :=
-  match goal with
-    [ Hx1: nullable ?g ?p _ (Some ?b1),
-      Hx2: nullable ?g ?p _ (Some ?b2) |- _ ] =>
+    [ Hx1: nullable ?g ?p ?b1,
+      Hx2: nullable ?g ?p ?b2 |- _ ] =>
           assert (b1 = b2)
-          by eauto using nullable_Some_determinism;
+          by eauto using nullable_determinism;
           clear Hx2
   end.
 
 Lemma verifyrule_similar_to_nullable :
   forall g p d b k,
   verifyrule g p d false (Some b) k ->
-  nullable g p d (Some b).
+  nullable g p b.
 Proof.
   intros * H.
   remember (Some b) as res.
@@ -362,53 +291,6 @@ Proof.
   eauto using nullable.
 Qed.
 
-Lemma nullable_none_is_verifyrule_none :
-  forall g p d,
-  (forall r, In r g -> coherent g r true) ->
-  coherent g p true ->
-  nullable g p d None ->
-  exists k, verifyrule g p d false None k.
-Proof.
-  intros * Hcg Hcp Hn.
-  remember None as res.
-  induction Hn;
-  inversion Hcp;
-  subst;
-  try discriminate;
-  try destruct2sep;
-  try match goal with
-    [ Hx: nth_error ?g ?i = Some ?p |- _ ] =>
-        assert (In p g)
-        by eauto using nth_error_In;
-        assert (coherent g p true)
-        by eauto
-  end;
-  repeat match goal with
-    [ IHx: (forall r, In r ?g -> coherent ?g ?p ?b) -> _,
-      Hx: forall r, In r ?g -> coherent ?g ?p ?b |- _ ] =>
-        specialize (IHx Hx)
-  end;
-  repeat specialize_coherent;
-  try specialize_eq_refl;
-  try destruct_exists_hyp;
-  eauto using verifyrule;
-  try (
-    assert (exists gas res k, verifyrule_comp g p1 d false gas = Some (res, k))
-    as [gas [res' [k Hvcp1]]]
-    by eauto using verifyrule_comp_termination;
-    assert (verifyrule g p1 d false res' k)
-    by eauto using verifyrule_comp_soundness;
-    destruct res';
-    eauto using verifyrule;
-    assert (nullable g p1 d (Some b))
-    by eauto using verifyrule_similar_to_nullable;
-    pose_nullable_determinism;
-    destruct1;
-    eauto using verifyrule;
-    fail
-  ).
-Qed.
-
 Lemma string_not_infinite :
   forall a s,
   String a s = s ->
@@ -418,14 +300,14 @@ Proof.
   induction s; congruence.
 Qed.
 
-Lemma nullable_Some_false_matches :
-  forall g p d,
-  nullable g p d (Some false) ->
+Lemma nullable_false_matches :
+  forall g p,
+  nullable g p false ->
   ~ exists s, matches g p s (Success s).
 Proof.
   intros * Hnullable [s Hmatches].
   generalize dependent s.
-  remember (Some false) as res.
+  remember false as b.
   induction Hnullable;
   intros;
   inversion Hmatches;
@@ -447,9 +329,9 @@ Proof.
   eauto using string_not_infinite.
 Qed.
 
-Lemma nullable_Some_false_proper_suffix :
-  forall g p d s s',
-  nullable g p d (Some false) ->
+Lemma nullable_false_proper_suffix :
+  forall g p s s',
+  nullable g p false ->
   matches g p s (Success s') ->
   proper_suffix s' s.
 Proof.
@@ -458,104 +340,43 @@ Proof.
   induction Hsuffix.
   - (* SuffixRefl *)
     exfalso.
-    eauto using (nullable_Some_false_matches _ _ _ Hnullable).
+    eauto using (nullable_false_matches _ _ Hnullable).
   - (* SuffixChar *)
     eauto using suffix_is_proper_suffix_with_char.
 Qed.
 
-Lemma nullable_convergence :
-  forall g p d d' res,
-  (forall r, In r g -> coherent g r true) ->
-  (forall r nb, In r g -> exists d b k, verifyrule g r d nb (Some b) k) ->
-  coherent g p true ->
-  length g < d ->
-  nullable g p d res ->
-  d <= d' ->
-  nullable g p d' res.
-Proof.
-  intros * Hgc Hgv Hpc Hlt H Hle.
-  assert (exists gas res k, verifyrule_comp g p d false gas = Some (res, k))
-  as [? [? [? ?]]]
-  by eauto using verifyrule_comp_termination.
-  match goal with
-    [ Hx: verifyrule_comp ?g ?p ?d false ?gas = Some (?res, ?k) |- _ ] =>
-        assert (verifyrule g p d false res k)
-        by eauto using verifyrule_comp_soundness
-  end.
-  assert (exists d b k, verifyrule g p d false (Some b) k)
-  as [? [? [? ?]]]
-  by eauto using verifyrule_safe_grammar_yields_safe_pattern.
-  match goal with
-    [ Hx: verifyrule ?g ?p ?d1 false (Some ?b) ?k1,
-      Hy: verifyrule ?g ?p ?d2 false ?res ?k2,
-      Hz: length ?g < ?d2 |- _ ] =>
-          destruct (Compare_dec.le_ge_dec d1 d2);
-          try match goal with
-            [ Hw: ?d1 <= ?d2,
-              Hv: length ?g < ?d2 |- _ ] =>
-                  assert (verifyrule g p d2 false (Some b) k1)
-                  by eauto using verifyrule_depth_le_some_determinism
-          end;
-          try match goal with
-            [ Hw: ?d1 >= ?d2 |- _ ] =>
-                assert (d2 <= d1) by lia;
-                assert (exists k', verifyrule g p d1 false res k')
-                as [? ?]
-                by eauto using verifyrule_convergence;
-                pose_verifyrule_determinism;
-                subst
-          end
-  end;
-  match goal with
-    [ Hx: nullable ?g ?p ?d ?res,
-      Hy: verifyrule ?g ?p ?d false (Some ?b) ?k |- _ ] =>
-          assert (nullable g p d (Some b))
-          by eauto using verifyrule_similar_to_nullable;
-          pose_nullable_determinism;
-          subst;
-          assert (exists k', verifyrule g p d' false (Some b) k')
-          as [? ?]
-          by eauto using verifyrule_convergence;
-          eauto using verifyrule_similar_to_nullable
-  end.
-Qed.
-
 (** Nullable function with gas **)
 
-Fixpoint nullable_comp g p d gas {struct gas} :=
+Fixpoint nullable_comp g p gas {struct gas} :=
   match gas with
   | O => None
   | S gas' => match p with
-              | PEmpty => Some (Some true)
-              | PSet _ => Some (Some false)
-              | PSequence p1 p2 => match nullable_comp g p1 d gas' with
-                                   | Some (Some true) => nullable_comp g p2 d gas'
+              | PEmpty => Some true
+              | PSet _ => Some false
+              | PSequence p1 p2 => match nullable_comp g p1 gas' with
+                                   | Some true => nullable_comp g p2 gas'
                                    | ob => ob
                                    end
-              | PChoice p1 p2 => match nullable_comp g p1 d gas' with
-                                 | Some (Some false) => nullable_comp g p2 d gas'
+              | PChoice p1 p2 => match nullable_comp g p1 gas' with
+                                 | Some false => nullable_comp g p2 gas'
                                  | ob => ob
                                  end
-              | PRepetition _ => Some (Some true)
-              | PNot _ => Some (Some true)
+              | PRepetition _ => Some true
+              | PNot _ => Some true
               | PNT i => match nth_error g i with
-                         | Some p' => match d with
-                                      | O => Some None
-                                      | S d' => nullable_comp g p' d' gas'
-                                      end
+                         | Some p' => nullable_comp g p' gas'
                          | None => None
                          end
               end
   end.
 
 Lemma nullable_comp_soundness :
-  forall g p d gas res,
-  nullable_comp g p d gas = Some res ->
-  nullable g p d res.
+  forall g p gas b,
+  nullable_comp g p gas = Some b ->
+  nullable g p b.
 Proof.
   intros * H.
-  generalize dependent res.
-  generalize dependent d.
+  generalize dependent b.
   generalize dependent p.
   generalize dependent g.
   induction gas; intros; try discriminate.
@@ -563,8 +384,8 @@ Proof.
   try (simpl in H; discriminate; fail);
   try (
     simpl in H;
-    try destruct (nullable_comp g p1 d gas)
-    as [[[|]|]|] eqn:?;
+    try destruct (nullable_comp g p1 gas)
+    as [[|]|] eqn:?;
     try discriminate;
     try destruct1;
     eauto using nullable;
@@ -574,24 +395,18 @@ Proof.
     simpl in H;
     destruct (nth_error g n) eqn:?;
     try discriminate;
-    try destruct1;
-    destruct d;
-    try discriminate;
-    try destruct1;
-    assert (In p g) as HIn by (eauto using nth_error_In);
     eauto using nullable;
     fail
   ).
 Qed.
 
 Lemma nullable_comp_S_gas :
-  forall g p d gas res,
-  nullable_comp g p d gas = Some res ->
-  nullable_comp g p d (S gas) = Some res.
+  forall g p gas b,
+  nullable_comp g p gas = Some b ->
+  nullable_comp g p (S gas) = Some b.
 Proof.
   intros * H.
-  generalize dependent res.
-  generalize dependent d.
+  generalize dependent b.
   generalize dependent p.
   generalize dependent g.
   induction gas; intros; try discriminate;
@@ -599,8 +414,8 @@ Proof.
   try destruct1;
   auto;
   try (
-    destruct (nullable_comp g p1 d gas) as [[[|]|]|] eqn:Hn1;
-    destruct (nullable_comp g p2 d gas) as [[[|]|]|] eqn:Hn2;
+    destruct (nullable_comp g p1 gas) as [[|]|] eqn:Hn1;
+    destruct (nullable_comp g p2 gas) as [[|]|] eqn:Hn2;
     try discriminate;
     destruct1;
     try apply IHgas in Hn1;
@@ -611,7 +426,7 @@ Proof.
     try destruct1;
     try discriminate;
     auto
-  ).
+  );
   try (
     destruct (nth_error g n) eqn:Hn;
     remember (S gas);
@@ -619,80 +434,189 @@ Proof.
     destruct_match_subject_in_goal;
     try destruct1;
     try discriminate;
-    auto;
-    destruct_match_subject_in_goal;
     auto
   ).
 Qed.
 
 Lemma nullable_comp_le_gas :
-  forall g p d gas1 gas2 res,
-  nullable_comp g p d gas1 = Some res ->
+  forall g p gas1 gas2 b,
+  nullable_comp g p gas1 = Some b ->
   gas1 <= gas2 ->
-  nullable_comp g p d gas2 = Some res.
+  nullable_comp g p gas2 = Some b.
 Proof.
   intros * H Hle.
   induction Hle;
   auto using nullable_comp_S_gas.
 Qed.
 
-(* Here, we could have used the max pat_size of the grammar
-   instead of summing up the pat_size of each rule of the grammar,
-   but the sum makes the proof of lower bound easier *)
-Lemma nullable_comp_gas_bounded :
-  forall g p d gas,
-  (forall r, In r g -> coherent g r true) ->
+Lemma nullable_comp_gas_exists :
+  forall g p d b k,
+  lcoherent g g true ->
   coherent g p true ->
-  gas >= pat_size p + d * (grammar_size g) ->
-  exists res, nullable_comp g p d gas = Some res.
+  verifyrule g p d false (Some b) k ->
+  exists gas, nullable_comp g p gas = Some b.
 Proof.
-  intros * Hgc Hpc Hge.
-  generalize dependent d.
-  generalize dependent p.
-  generalize dependent g.
-  induction gas; intros;
-  try (destruct p; inversion Hge; fail);
-  destruct p;
+  intros * Hgc Hpc Hpv.
+  remember false as nb.
+  remember (Some b) as res.
+  generalize dependent b.
+  induction Hpv; intros;
   inversion Hpc; subst;
-  try (simpl; eauto; fail);
-  try (
-    simpl in Hge;
-    assert (gas >= pat_size p1 + d * grammar_size g) by lia;
-    assert (gas >= pat_size p2 + d * grammar_size g) by lia;
-    assert (exists res, nullable_comp g p1 d gas = Some res) as [res1 Hn1] by auto;
-    assert (exists res, nullable_comp g p2 d gas = Some res) by auto;
-    simpl;
-    rewrite Hn1;
-    destruct res1 as [[|]|];
-    eauto;
-    fail
-  );
-  try (
-    simpl in Hge;
-    simpl;
+  try discriminate;
+  try destruct1;
+  try (assert (b = true) by eauto using verifyrule_true_res_some_true; subst);
+  try (exists 1; simpl; eauto; fail).
+  - (* PSequence p1 p2, where p1 is nullable *)
+    assert (exists gas, nullable_comp g p1 gas = Some true)
+    as [gas1 ?] by eauto.
+    assert (exists gas, nullable_comp g p2 gas = Some b)
+    as [gas2 ?] by eauto.
+    pose (gas1 + gas2) as gas.
+    assert (gas1 <= gas) by lia.
+    assert (gas2 <= gas) by lia.
+    assert (nullable_comp g p1 gas = Some true)
+    by eauto using nullable_comp_le_gas.
+    assert (nullable_comp g p2 gas = Some b)
+    by eauto using nullable_comp_le_gas.
+    exists (S gas).
+    simpl.
+    rewrite_match_subject_in_goal.
+    auto.
+  - (* PSequence p1 p2, where p1 is non-nullable *)
+    assert (exists gas, nullable_comp g p1 gas = Some false)
+    as [gas ?] by eauto.
+    exists (S gas).
+    simpl.
+    rewrite_match_subject_in_goal.
+    auto.
+  - (* PChoice p1 p2 *)
+    assert (exists gas, nullable_comp g p1 gas = Some nb')
+    as [gas1 ?] by eauto.
+    destruct nb'.
+    + (* p1 is nullable *)
+      exists (S gas1).
+      simpl.
+      rewrite_match_subject_in_goal.
+      assert (b = true)
+      by eauto using verifyrule_true_res_some_true.
+      subst.
+      auto.
+    + (* p1 is non-nullable *)
+      assert (exists gas, nullable_comp g p2 gas = Some b)
+      as [gas2 ?] by eauto.
+      pose (gas1 + gas2) as gas.
+      assert (gas1 <= gas) by lia.
+      assert (gas2 <= gas) by lia.
+      assert (nullable_comp g p1 gas = Some false)
+      by eauto using nullable_comp_le_gas.
+      assert (nullable_comp g p2 gas = Some b)
+      by eauto using nullable_comp_le_gas.
+      exists (S gas).
+      simpl.
+      rewrite_match_subject_in_goal.
+      auto.
+  - (* PNT i *)
+    destruct2sep.
     match goal with
-      [ Hx: ?lhs = _ |-
-        exists _, match ?lhs with | _ => _ end = _ ] =>
-          rewrite Hx
-    end;
-    assert (In p g) as HIn by (eauto using nth_error_In);
-    destruct d; eauto;
-    specialize (pat_size_le_grammar_size _ _ HIn) as Hle;
-    assert (gas >= pat_size p + d * grammar_size g) by lia;
-    auto;
-    fail
-  ).
+      [ Hx: nth_error _ _ = Some ?p |- _ ] =>
+          assert (In p g) by eauto using nth_error_In;
+          assert (coherent g p true) by eauto using lcoherent_true_In;
+          assert (exists gas, nullable_comp g p gas = Some b)
+          as [gas ?] by eauto;
+          exists (S gas);
+          simpl;
+          rewrite Hx;
+          auto
+    end.
 Qed.
 
-(* Here, we don't care about any particular lower bound value.
-   We just know there exists SOME gas for which nullable_comp
-   gives SOME result. :-) *)
-Lemma nullable_comp_termination :
-  forall g p d,
-  (forall r, In r g -> coherent g r true) ->
+Lemma nullable_comp_gas_bounded_by_depth :
+  forall g p d b k gas,
+  lcoherent g g true ->
   coherent g p true ->
-  exists gas b,
-  nullable_comp g p d gas = Some b.
+  verifyrule g p d false (Some b) k ->
+  gas >= pat_size p + d * (grammar_size g) ->
+  nullable_comp g p gas = Some b.
 Proof.
-  eauto using nullable_comp_gas_bounded.
+  intros * Hlc Hc Hv Hge.
+  generalize dependent gas.
+  remember false as nb.
+  remember (Some b) as res.
+  generalize dependent b.
+  induction Hv; intros;
+  inversion Hc; subst;
+  try destruct1;
+  simpl in Hge;
+  destruct gas;
+  try match goal with
+    [ Hx: 0 >= S _ |- _ ] =>
+        inversion Hx
+  end;
+  try discriminate;
+  eauto.
+  - (* PSequence p1 p2, where p1 is nullable *)
+    assert (gas >= pat_size p1 + d * (grammar_size g)) by lia.
+    assert (gas >= pat_size p2 + d * (grammar_size g)) by lia.
+    assert (nullable_comp g p1 gas = Some true) by eauto.
+    simpl.
+    rewrite_match_subject_in_goal.
+    eauto.
+  - (* PSequence p1 p2, where p1 is non-nullable *)
+    assert (gas >= pat_size p1 + d * (grammar_size g)) by lia.
+    assert (nullable_comp g p1 gas = Some false) by eauto.
+    simpl.
+    rewrite_match_subject_in_goal.
+    eauto.
+  - (* PChoice p1 p2 *)
+    assert (gas >= pat_size p1 + d * (grammar_size g)) by lia.
+    assert (gas >= pat_size p2 + d * (grammar_size g)) by lia.
+    assert (nullable_comp g p1 gas = Some nb') by eauto.
+    simpl.
+    rewrite_match_subject_in_goal.
+    destruct nb'.
+    + (* p1 is nullable *)
+      assert (b = true)
+      by eauto using verifyrule_true_res_some_true.
+      subst.
+      eauto.
+    + (* p1 is non-nullable *)
+    assert (gas >= pat_size p2 + d * (grammar_size g)) by lia.
+    eauto.
+  - (* PRepetition p *)
+    assert (b = true)
+    by eauto using verifyrule_true_res_some_true.
+    subst.
+    simpl.
+    eauto.
+  - (* PNot p *)
+    assert (b = true)
+    by eauto using verifyrule_true_res_some_true.
+    subst.
+    simpl.
+    eauto.
+  - (* PNT i *)
+    destruct2sep.
+    simpl.
+    rewrite_match_subject_in_goal.
+    match goal with
+      [ Hx: nth_error ?g _ = Some ?p |- _ ] =>
+        assert (pat_size p <= grammar_size g)
+        by eauto using pat_size_le_grammar_size, nth_error_In;
+        assert (gas >= pat_size p + d * (grammar_size g)) by lia
+    end.
+    eauto using lcoherent_true_In, nth_error_In.
+Qed.
+
+Lemma nullable_comp_gas_bounded :
+  forall g p d b k gas,
+  lcoherent g g true ->
+  coherent g p true ->
+  verifyrule g p d false (Some b) k ->
+  gas >= pat_size p + S (Datatypes.length g) * (grammar_size g) ->
+  nullable_comp g p gas = Some b.
+Proof.
+  intros.
+  assert (exists k', verifyrule g p (S (Datatypes.length g)) false (Some b) k')
+  as [? ?] by eauto using verifyrule_Some_min_depth.
+  eauto using nullable_comp_gas_bounded_by_depth.
 Qed.
