theories/Verifygrammar.v
@@ -131,7 +131,7 @@ Proof.
   eauto using verifygrammar_comp_S_gas.
 Qed.
 
-Lemma verifygrammar_comp_termination :
+Lemma verifygrammar_comp_gas_exists :
   forall g,
   exists gas b,
   verifygrammar_comp g gas = Some b.
@@ -143,14 +143,14 @@ Proof.
   + (* true *)
     assert (exists gas b, lverifyrule_comp g g gas = Some b)
     as [gasv [bv Hv]]
-    by eauto using lverifyrule_comp_termination.
+    by eauto using lverifyrule_comp_gas_exists.
     assert (lverifyrule g g bv)
     by eauto using lverifyrule_comp_soundness.
     destruct bv.
     - (* true *)
       assert (exists gas b, lcheckloops_comp g g gas = Some b)
       as [gasl [bl Hl]]
-      by eauto using lcheckloops_comp_termination.
+      by eauto using lcheckloops_comp_gas_exists.
       assert (lcheckloops g g bl)
       by eauto using lcheckloops_comp_soundness.
       pose (gasv + gasl) as gas.
@@ -220,16 +220,16 @@ Inductive verifygrammarpat : grammar -> pat -> bool -> Prop :=
       coherent g p false ->
       verifygrammarpat g p false
   | VGPPatWithEmptyLoop :
-      forall g p d,
+      forall g p,
       verifygrammar g true ->
       coherent g p true ->
-      checkloops g p d (Some true) ->
+      checkloops g p true ->
       verifygrammarpat g p false
   | VGPSafe :
-      forall g p d,
+      forall g p,
       verifygrammar g true ->
       coherent g p true ->
-      checkloops g p d (Some false) ->
+      checkloops g p false ->
       verifygrammarpat g p true
   .
 
@@ -247,16 +247,16 @@ Proof.
   eauto using verifygrammar_determinism,
               coherent_determinism,
               checkloops_determinism,
-              checkloops_Some_determinism.
+              checkloops_determinism.
 Qed.
 
 Definition verifygrammarpat_comp g p gas :=
   match verifygrammar_comp g gas with
   | Some true => match coherent_func g p with
-                 | true => match checkloops_comp g p (S (length g)) gas with
-                           | Some (Some false) => Some true
-                           | Some (Some true) => Some false
-                           | _ => None
+                 | true => match checkloops_comp g p gas with
+                           | Some false => Some true
+                           | Some true => Some false
+                           | None => None
                            end
                  | false => Some false
                  end
@@ -298,9 +298,9 @@ Proof.
         )
   end;
   try match goal with
-    [ Hx: checkloops_comp ?g ?p ?d ?gas = Some ?b |- _ ] =>
+    [ Hx: checkloops_comp ?g ?p ?gas = Some ?b |- _ ] =>
         let H := fresh in (
-          assert (checkloops_comp g p d (S gas) = Some b)
+          assert (checkloops_comp g p (S gas) = Some b)
           as H
           by eauto using checkloops_comp_S_gas;
           rewrite H;
@@ -320,7 +320,7 @@ Proof.
   eauto using verifygrammarpat_comp_S_gas.
 Qed.
 
-Lemma verifygrammarpat_comp_termination :
+Lemma verifygrammarpat_comp_gas_exists :
   forall g p,
   exists gas b,
   verifygrammarpat_comp g p gas = Some b.
@@ -329,7 +329,7 @@ Proof.
   unfold verifygrammarpat_comp.
   assert (exists gas b, verifygrammar_comp g gas = Some b)
   as [gasvg [bvg Hvgc]]
-  by eauto using verifygrammar_comp_termination.
+  by eauto using verifygrammar_comp_gas_exists.
   assert (verifygrammar g bvg)
   as Hvg
   by eauto using verifygrammar_comp_soundness.
@@ -339,32 +339,24 @@ Proof.
     destruct (coherent_func g p) eqn:Hcp;
     apply coherent_func_soundness in Hcp as ?.
     + (* true *)
-      pose (S (length g)) as d.
-      assert (exists gas b, checkloops_comp g p d gas = Some b)
-      as [gasl [rescl ?]]
-      by eauto using checkloops_comp_termination, lcoherent_true_In.
-      assert (checkloops g p d rescl)
+      assert (exists gas b, checkloops_comp g p gas = Some b)
+      as [gascl [bcl ?]]
+      by eauto using checkloops_comp_gas_exists.
+      assert (checkloops g p bcl)
       by eauto using checkloops_comp_soundness.
-      assert (exists d b, checkloops g p d (Some b))
-      as [d' [bl' ?]]
-      by eauto using checkloops_safe_grammar, lcoherent_true_In, lverifyrule_true_In.
-      assert (rescl = Some bl')
-      by eauto using checkloops_Some_convergence, lcoherent_true_In, lverifyrule_true_In.
-      subst rescl.
-      pose (gasvg + gasl) as gas.
+      pose (gasvg + gascl) as gas.
       assert (gasvg <= gas) by lia.
-      assert (gasl <= gas) by lia.
+      assert (gascl <= gas) by lia.
       exists gas.
       assert (verifygrammar_comp g gas = Some true)
       as Hv'
       by eauto using verifygrammar_comp_le_gas.
       rewrite Hv'.
-      assert (checkloops_comp g p d gas = Some (Some bl'))
+      assert (checkloops_comp g p gas = Some bcl)
       as Hl'
       by eauto using checkloops_comp_le_gas.
-      subst d.
       rewrite Hl'.
-      destruct bl';
+      destruct bcl;
       eauto.
     + (* false *)
       exists gasvg.
@@ -402,17 +394,12 @@ Proof.
   assert (coherent g p true)
   by eauto using coherent_func_soundness.
   assert (gas >= pat_size p + S (length g) * grammar_size g) by lia.
-  assert (exists b, checkloops_comp g p (S (length g)) gas = Some b)
+  assert (exists b, checkloops_comp g p gas = Some b)
   as [rescl Hcl] by eauto using checkloops_comp_gas_bounded, lcoherent_true_In.
-  assert (exists d b, checkloops g p d (Some b))
-  as [d [b ?]]
-  by eauto using checkloops_safe_grammar, lcoherent_true_In, lverifyrule_true_In.
-  assert (checkloops g p (S (length g)) rescl)
+  assert (checkloops g p rescl)
   by eauto using checkloops_comp_soundness.
-  assert (rescl = Some b)
-  by eauto using checkloops_Some_convergence, lcoherent_true_In, lverifyrule_true_In.
   rewrite Hcl.
-  destruct rescl as [[|]|]; eauto.
+  destruct rescl; eauto.
 Qed.
 
 Definition verifygrammarpat_func g p :=
@@ -443,18 +430,17 @@ Proof.
 Qed.
 
 Theorem safe_match :
-  forall g p d s,
+  forall g p s,
   (forall r, In r g -> coherent g r true) ->
   (forall r nb, In r g -> exists d b k, verifyrule g r d nb (Some b) k) ->
-  (forall r, In r g -> exists d, checkloops g r d (Some false)) ->
+  (forall r, In r g -> checkloops g r false) ->
   coherent g p true ->
-  checkloops g p d (Some false) ->
+  checkloops g p false ->
   exists res, matches g p s res.
 Proof.
   intros * Hcg Hvg Hclg Hcp Hclp.
   remember (String.length s) as n.
   generalize dependent s.
-  generalize dependent d.
   generalize dependent p.
   generalize dependent g.
   induction n using strong_induction;
@@ -465,7 +451,6 @@ Proof.
   remember (Some b) as res in Hvp.
   generalize dependent b.
   generalize dependent s.
-  generalize dependent d.
   generalize dependent n.
   induction Hvp;
   intros;
@@ -506,7 +491,7 @@ Proof.
   - (* PSequence p1 p2, with non-nullable p1 *)
     match goal with
       [ _: verifyrule ?g p1 ?d false (Some false) _ |- _ ] =>
-          assert (nullable g p1 d (Some false))
+          assert (nullable g p1 false)
           by eauto using verifyrule_similar_to_nullable
     end.
     assert (exists res, matches g p1 s res) as [res1 ?] by eauto.
@@ -516,7 +501,7 @@ Proof.
     as [? ?]
     by eauto using
     proper_suffix_length_lt,
-    nullable_Some_false_proper_suffix.
+    nullable_false_proper_suffix.
     eauto using matches.
   - (* PChoice p1 p2 *)
     assert (exists res, matches g p1 s res) as [res1 ?] by eauto.
@@ -532,7 +517,7 @@ Proof.
     as [? ?]
     by eauto using
     proper_suffix_length_lt,
-    nullable_Some_false_proper_suffix.
+    nullable_false_proper_suffix.
     eauto using matches.
   - (* PNot p *)
     assert (exists res, matches g p s res) as [res ?] by eauto.
@@ -540,29 +525,28 @@ Proof.
     eauto using matches.
   - (* PNT i *)
     assert (In p g) by eauto using nth_error_In.
-    assert (exists d, checkloops g p d (Some false))
-    as [? ?] by eauto.
+    assert (checkloops g p false) by eauto.
     assert (exists res, matches g p s res) as [? ?] by eauto.
     eauto using matches.
 Qed.
 
 Theorem lpredicates_safe_match :
-  forall g p d s,
+  forall g p s,
   lcoherent g g true ->
   lverifyrule g g true ->
   lcheckloops g g false ->
   coherent g p true ->
-  checkloops g p d (Some false) ->
+  checkloops g p false ->
   exists res, matches g p s res.
 Proof.
   eauto using safe_match, lcoherent_true_In, lverifyrule_true_In, lcheckloops_false_In.
 Qed.
 
 Theorem verifygrammar_safe_match :
-  forall g p d s,
+  forall g p s,
   verifygrammar g true ->
   coherent g p true ->
-  checkloops g p d (Some false) ->
+  checkloops g p false ->
   exists res, matches g p s res.
 Proof.
   intros * Hvg Hpc Hlp.
